Made current Phase1 invariant inductive across steps of non-leaders

ironfleet/src/Dafny/Distributed/Protocol/RSL/PerformanceProof/PerformanceProof.i.dfy
@@ -25,6 +25,7 @@ predicate RslAssumption(s:TimestampedRslState)
 predicate RslConsistency(s:TimestampedRslState)
 {
   ConstantsAllConsistentInv(UntimestampRslState(s))
+    && WellFormedLConfiguration(s.constants.config)
 }
 
 predicate ViewAlwaysZero(s:TimestampedRslState)
@@ -67,7 +68,8 @@ predicate InitInvariant(s:TimestampedRslState)
   && (0 < |s.t_replicas| ==>
   var p := s.t_replicas[0].v.replica.proposer;
     && p.current_state == 0
-    && BalLt(p.max_ballot_i_sent_1a, p.election_state.current_view)
+    && p.election_state.current_view == Ballot(1, 0)
+    && p.max_ballot_i_sent_1a == Ballot(0, 0)
   )
 
   && (forall idx :: 0 <= idx < |s.t_replicas|
@@ -91,6 +93,11 @@ predicate Phase1Invariant(s:TimestampedRslState)
   && s.t_replicas[idx].v.replica.learner.unexecuted_learner_state == map[]
   )
 
+  && (forall idx :: 0 < idx < |s.t_replicas|
+  ==>
+  && s.t_replicas[idx].v.replica.proposer.current_state == 0
+  )
+
   && (0 < |s.t_replicas| ==>
     && TimeLe(s.t_replicas[0].ts, TimeBound1aSent())
   )
@@ -102,23 +109,32 @@ predicate Phase1Invariant(s:TimestampedRslState)
   ==>
    || pkt.msg.v.RslMessage_Heartbeat?
    || pkt.msg.v.RslMessage_1a?
+   || pkt.msg.v.RslMessage_1b?
+  )
+
+  && (forall pkt :: pkt in s.t_environment.sentPackets
+  && pkt.msg.v.RslMessage_1b?
+  ==> pkt.dst == s.constants.config.replica_ids[0]
   )
 
   && (forall pkt :: pkt in s.t_environment.sentPackets
       && pkt.msg.v.RslMessage_1a?
-      && |s.t_replicas| > 0
    ==> TimeLe(pkt.msg.ts, TimeBound1aSent())
-      && pkt.msg.v.bal_1a == s.t_replicas[0].v.replica.proposer.max_ballot_i_sent_1a
+      && (|s.t_replicas| > 0 ==> pkt.msg.v.bal_1a == s.t_replicas[0].v.replica.proposer.max_ballot_i_sent_1a)
+      && pkt.msg.v.bal_1a == Ballot(1, 0)
+      && pkt.src == s.constants.config.replica_ids[0]
   )
 
   && (forall idx :: 0 < idx < |s.t_replicas|
   ==>
-  if s.t_replicas[idx].v.replica.acceptor.max_bal == Ballot(0, 0) then
-    // TODO: s.t_replicas[idx].ts == TimeZero() 
-    true
-  else
-    (&& s.t_replicas[idx].v.replica.acceptor.max_bal == s.t_replicas[0].v.replica.proposer.max_ballot_i_sent_1a
-    && s.t_replicas[idx].ts == TimeBound1aReceived())
+  (s.t_replicas[idx].v.replica.acceptor.max_bal == Ballot(0, 0)
+  ==>
+  LSchedulerTimeBound(s.t_replicas[idx])
+  )
+  //else
+    //(&& s.t_replicas[idx].v.replica.acceptor.max_bal == s.t_replicas[0].v.replica.proposer.max_ballot_i_sent_1a
+    //&& true // TimeLe(s.t_replicas[idx].ts, TimeBound1aReceived())
+    //)
   )
 }
 
@@ -127,51 +143,41 @@ lemma lemma_RslInitImpliesInitInv(s:TimestampedRslState)
   requires TimestampedRslInit(s.constants, s);
   ensures InitInvariant(s);
 {
-  
 }
 
-lemma lemma_not1_0_InitGoesToInit(s:TimestampedRslState, s':TimestampedRslState)
+lemma lemma_0_1_InitGoesToPhase1(s:TimestampedRslState, s':TimestampedRslState, j:int)
   requires RslAssumption(s);
   requires ViewAlwaysZero(s)
   requires RslConsistency(s);
   requires RslConsistency(s');
+  requires 0 == j < |s.constants.config.replica_ids|
 
   requires s.t_environment.nextStep.LEnvStepHostIos?;
-  requires s.t_environment.nextStep.actor == s.constants.config.replica_ids[0];
-  requires s.t_environment.nextStep.nodeStep != RslStep(1);
-
-  requires TimestampedRslNextOneReplica(s, s', 0, s.t_environment.nextStep.ios);
-
-  requires InitInvariant(s)
-  ensures InitInvariant(s')
-{
-}
-
-lemma lemma_1_0_InitGoesToPhase1(s:TimestampedRslState, s':TimestampedRslState)
-  requires RslAssumption(s);
-  requires ViewAlwaysZero(s)
-  requires RslConsistency(s);
-  requires RslConsistency(s');
-
-  requires s.t_environment.nextStep.LEnvStepHostIos?;
-  requires s.t_environment.nextStep.actor == s.constants.config.replica_ids[0];
+  requires s.t_environment.nextStep.actor == s.constants.config.replica_ids[j];
   requires s.t_environment.nextStep.nodeStep == RslStep(1);
 
-  requires TimestampedRslNextOneReplica(s, s', 0, s.t_environment.nextStep.ios);
+  requires TimestampedRslNextOneReplica(s, s', j, s.t_environment.nextStep.ios);
 
   requires InitInvariant(s)
   ensures Phase1Invariant(s')
 {
+  forall pkt | pkt in s'.t_environment.sentPackets
+      && pkt.msg.v.RslMessage_1a?
+  {
+    assert TimeLe(pkt.msg.ts, TimeBound1aSent());
+    assert pkt.msg.v.bal_1a == s'.t_replicas[0].v.replica.proposer.max_ballot_i_sent_1a;
+    assert BalLt(Ballot(0, 0), pkt.msg.v.bal_1a);
+    assert pkt.src == s.constants.config.replica_ids[0];
+  }
+
 }
 
-lemma lemma_a_j_InitGoesToInit(s:TimestampedRslState, s':TimestampedRslState, j:int)
+lemma lemma_InitGoesToInitOrPhase1(s:TimestampedRslState, s':TimestampedRslState, j:int)
   requires RslAssumption(s);
   requires ViewAlwaysZero(s)
   requires RslConsistency(s);
   requires RslConsistency(s');
   requires 0 <= j < |s.constants.config.replica_ids|
-
-  requires j > 0;
 
   requires s.t_environment.nextStep.LEnvStepHostIos?;
   requires s.t_environment.nextStep.actor == s.constants.config.replica_ids[j];
@@ -179,8 +185,17 @@ lemma lemma_a_j_InitGoesToInit(s:TimestampedRslState, s':TimestampedRslState, j:
   requires TimestampedRslNextOneReplica(s, s', j, s.t_environment.nextStep.ios);
 
   requires InitInvariant(s)
-  ensures InitInvariant(s')
+  ensures InitInvariant(s') || Phase1Invariant(s')
 {
+  if (s.t_replicas[0].v.nextActionIndex == 1) {
+    if (j == 0) {
+        assert Phase1Invariant(s');
+    } else {
+        assert InitInvariant(s');
+    }
+  } else {
+    assert InitInvariant(s');
+  }
 }
 
 lemma lemma_a_j_Phase1GoesToPhase1(s:TimestampedRslState, s':TimestampedRslState, j:int)
@@ -200,6 +215,7 @@ lemma lemma_a_j_Phase1GoesToPhase1(s:TimestampedRslState, s':TimestampedRslState
   requires Phase1Invariant(s)
   ensures Phase1Invariant(s')
 {
+  assert ReplicasDistinct(s.constants.config.replica_ids, 0, j);
 }
 
 }
